Some more progress on inject/extract, prove full abstraction using some admitted results.

BackTrans/Emulate.v
@@ -1,6 +1,7 @@
 Require Stlc.SpecSyntax.
 Require Utlc.SpecSyntax.
 Require Import BackTrans.UValHelpers.
+Require Import BackTrans.UValHelpers2.
 Require Import Stlc.SpecTyping.
 Require Import Stlc.StlcOmega.
 Require Import Stlc.LemmasTyping.
@@ -21,43 +22,6 @@ Require Import Db.Lemmas.
 Require Import UVal.UVal.
 Require Utlc.Fix.
 Require Omega.
-
-Definition uvalApp_pctx₁ n ts₂ := S.papp₁ (S.papp₂ (S.abs (UVal n) (S.abs (UVal n) (S.app (caseArrUp n (S.var 1)) (S.var 0)))) S.phole) ts₂.
-Definition uvalApp_pctx₂ n ts₁ := S.papp₂ (S.app (S.abs (UVal n) (S.abs (UVal n) (S.app (caseArrUp n (S.var 1)) (S.var 0)))) ts₁) S.phole.
-Definition uvalApp n ts₁ ts₂ := S.app (S.app (S.abs (UVal n) (S.abs (UVal n) (S.app (caseArrUp n (S.var 1)) (S.var 0)))) ts₁) ts₂.
-
-(* Arguments uvalApp_pctx₁ n ts₂ : simpl never. *)
-(* Arguments uvalApp_pctx₂ n ts₁ : simpl never. *)
-(* Arguments uvalApp n ts₁ ts₂ : simpl never. *)
-
-Lemma uvalApp_T {n ts₁ ts₂ Γ} :
-  ⟪ Γ ⊢ ts₁ : UVal n ⟫ →
-  ⟪ Γ ⊢ ts₂ : UVal n ⟫ →
-  ⟪ Γ ⊢ uvalApp n ts₁ ts₂ : UVal n ⟫.
-Proof.
-  unfold uvalApp.
-  eauto with typing uval_typing.
-Qed.
-
-Lemma uvalApp_pctx₁_T {n ts₂ Γ} :
-  ⟪ Γ ⊢ ts₂ : UVal n ⟫ →
-  ⟪ ⊢ uvalApp_pctx₁ n ts₂ : Γ , UVal n → Γ , UVal n ⟫.
-Proof.
-  unfold uvalApp_pctx₁.
-  eauto with typing uval_typing.
-Qed.
-
-Lemma uvalApp_pctx₂_T {n ts₁ Γ} :
-  ⟪ Γ ⊢ ts₁ : UVal n ⟫ →
-  ⟪ ⊢ uvalApp_pctx₂ n ts₁ : Γ , UVal n → Γ , UVal n ⟫.
-Proof.
-  unfold uvalApp_pctx₂.
-  eauto with typing uval_typing.
-Qed.
-
-Hint Resolve uvalApp_T : uval_typing.
-Hint Resolve uvalApp_pctx₁_T : uval_typing.
-Hint Resolve uvalApp_pctx₂_T : uval_typing.
 
 Fixpoint emulate (n : nat) (t : U.UTm) : S.Tm :=
   match t with
@@ -273,98 +237,6 @@ Qed.
 (*     eauto using compat_emul_abs. *)
 (* Qed. *)
 
-Lemma termrel_uvalApp {d w n p ts₁ tu₁ ts₂ tu₂} :
-  dir_world_prec n w d p →
-  termrel d w (pEmulDV n p) ts₁ tu₁ →
-  (∀ w' : World, w' ≤ w → termrel d w' (pEmulDV n p) ts₂ tu₂) →
-  termrel d w (pEmulDV n p) (uvalApp n ts₁ ts₂) (U.app tu₁ tu₂).
-Proof.
-  intros dwp tr₁ tr₂.
-  unfold uvalApp, caseArrUp, caseArrUp_pctx.
-  (* evaluate ts₁ and tu₁ *)
-  eapply (termrel_ectx' tr₁); S.inferContext; U.inferContext; 
-  unfold pctx_cat, U.ECtx; crush.
-
-  (* continuation boilerplate *)
-  intros w' futw vs₁ vu₁ vr₁.
-  destruct (valrel_implies_OfType vr₁) as [[vvs₁ ?] [? ?]].
-  rewrite S.pctx_cat_app; cbn.
-
-  (* beta-reduce the outer let *)
-  eapply termrel_antired_eval_left.
-  eapply (S.eval_from_eval₀ (S.eval_beta vvs₁)); S.inferContext; crush.
-  cbn; crush.
-
-  (* bureaucracy *)
-  fold (caseArr n (S.app (upgrade n 1) (S.var 1))).
-  rewrite caseArr_sub; cbn; crush; rewrite upgrade_sub.
-
-  (* evaluate ts₂ and tu₂ *)
-  specialize (tr₂ w' futw).
-  eapply (termrel_ectx' tr₂); S.inferContext; U.inferContext; 
-  unfold pctx_cat, U.ECtx; crush.
-  
-  (* continuation boilerplate *)
-  intros w'' futw' vs₂ vu₂ vr₂.
-  destruct (valrel_implies_Value vr₂) as [vvs₂ ?].
-  cbn.
-
-  (* beta-reduce the remaining let *)
-  eapply termrel_antired_eval_left.
-  eapply (S.eval_from_eval₀ (S.eval_beta vvs₂)); S.inferContext; crush.
-  cbn; crush.
-
-  (* bureaucracy *)
-  fold (caseArr n (S.app (upgrade n 1) (S.var 1))).
-  rewrite ?caseArr_sub; cbn; crush; rewrite ?upgrade_sub.
-  rewrite <- ?ap_liftSub; rewrite -> ?liftSub_wkm; rewrite (apply_wkm_beta1_cancel vs₁ vs₂).
-  
-  (* execute the upgrade *)
-  assert (w'' ≤ w) by Omega.omega.
-  assert (valrel d w'' (pEmulDV n p) vs₁ vu₁) by eauto using valrel_mono.
-  assert (trupg : termrel d w'' (pEmulDV (n + 1) p) (S.app (upgrade n 1) vs₁) vu₁)
-    by (eauto using upgrade_works', dwp_mono).
-  unfold caseArr.
-  eapply (termrel_ectx' trupg); S.inferContext; U.inferContext; cbn; crush.
-
-  (* continuation bureaucracy *)
-  intros w''' futw'' vs₁' vu₁' vr₁'.
-  replace (n + 1) with (S n) in vr₁' by Omega.omega.
-
-  destruct (valrel_implies_Value vr₁').
-  (* case analysis *)
-  eapply invert_valrel_pEmulDV_for_caseUValArr in vr₁'.
-  destruct vr₁' as [(vs₁'' & ? & es & vr₁')|[(? & div)|(neq & div)]]; subst.
-  - (* Correct case *)
-
-    (* caseArr succeeds *)
-    eapply termrel_antired_star_left.
-    fold (caseArr n (inArr n vs₁'')).
-    eapply (evalstar_ctx' es); S.inferContext; crush.
-    cbn.
-
-    (* application works *)
-    eapply valrel_in_termrel in vr₁'.
-    eapply (termrel_app vr₁').
-
-    (* application argument is also fine *)
-    eauto using valrel_in_termrel, valrel_mono.
-  - (* unk case *) 
-    eapply dwp_imprecise in dwp; subst.
-    eapply termrel_div_lt.
-    fold (caseArr n vs₁').
-    eapply (divergence_closed_under_evalcontext' div); S.inferContext; crush.
-  - (* other cases *)
-    
-    eapply termrel_div_wrong.
-    + fold (caseArr n vs₁').
-      eapply (divergence_closed_under_evalcontext' div); S.inferContext; crush.
-    + right.
-      eapply evalToStar.
-      eapply U.eval₀_to_eval.
-      eauto with eval.
-Qed.
-
 Lemma compat_emul_pair {n m d p Γ ts₁ tu₁ ts₂ tu₂} :
   dir_world_prec n m d p →
   ⟪ Γ ⊩ ts₁ ⟦ d , m ⟧ tu₁ : pEmulDV n p ⟫ →
@@ -436,7 +308,7 @@ Proof.
     + intros w''' vs₂' vu₂' fw'' vr₂. eapply tr₂; eauto with arith.
     + intros w''' vs₃' vu₃' fw'' vr₃. eapply tr₃; eauto with arith.
   - (* unk case *)
-    eapply dwp_imprecise in dwp; subst.
+    eapply dwp_invert_imprecise in dwp; subst.
     eapply termrel_div_lt.
     eapply (divergence_closed_under_evalcontext' div); S.inferContext; crush.
   - (* other cases *)
@@ -516,7 +388,7 @@ Proof.
     + intros w''' fw''. eapply tr₂; Omega.omega.
     + intros w''' fw''. eapply tr₃; Omega.omega.
   - (* unk case *)
-    eapply dwp_imprecise in dwp; subst.
+    eapply dwp_invert_imprecise in dwp; subst.
     eapply termrel_div_lt.
     eapply (divergence_closed_under_evalcontext' div); S.inferContext; crush.
   - (* other cases *)
@@ -570,7 +442,7 @@ Proof.
     with (S.app (caseArrUp n ts₁) [γs] ts₂[γs]).
     change (U.app tu₁ tu₂)[γu] with (U.app tu₁[γu] tu₂[γu]).
     cbn; crush.
-    rewrite caseArrUp_sub; cbn; crush.
+    rewrite uvalApp_sub; cbn; crush.
     change (wk 0) with 1.
 
     eapply termrel_uvalApp; eauto.
@@ -618,7 +490,7 @@ Proof.
     + eauto using valrel_in_termrel, valrel_unit.
     + intros; eapply tr₂; eauto with arith.
   - (* unk case *)
-    eapply dwp_imprecise in dwp; subst.
+    eapply dwp_invert_imprecise in dwp; subst.
     eapply termrel_div_lt.
     eapply (divergence_closed_under_evalcontext' div); S.inferContext; crush.
   - (* other cases *)
@@ -662,7 +534,8 @@ Proof.
   eapply (termrel_ectx' tr); S.inferContext; U.inferContext; crush;
   eauto using inSumDwn_pctx_ectx. 
   intros w' fw vs vu vr.
-  eapply termrel_inSumDwn; simpl; eauto using valrel_inl, dwp_mono.
+  eapply termrel₀_in_termrel.
+  eapply termrel₀_inSumDwn; simpl; eauto using valrel_inl, dwp_mono.
 Qed.
 
 Lemma compat_emul_inl {n m d p Γ ts tu} :
@@ -690,7 +563,8 @@ Proof.
   eapply (termrel_ectx' tr); S.inferContext; U.inferContext; crush;  
   eauto using inSumDwn_pctx_ectx. 
   intros w' fw vs vu vr.
-  eapply termrel_inSumDwn; simpl; eauto using valrel_inr, dwp_mono.
+  eapply termrel₀_in_termrel.
+  eapply termrel₀_inSumDwn; simpl; eauto using valrel_inr, dwp_mono.
 Qed.
 
 Lemma compat_emul_inr {n m d p Γ ts tu} :
@@ -742,7 +616,7 @@ Proof.
     eapply (evalstar_ctx' es); S.inferContext; crush.
     simpl.
     eauto using termrel_proj₁, valrel_in_termrel.
-  - subst; eapply dwp_imprecise in dwp; subst.
+  - subst; eapply dwp_invert_imprecise in dwp; subst.
     eapply termrel_div_lt.
     eapply (divergence_closed_under_evalcontext' div); S.inferContext; crush.
   - eapply termrel_div_wrong.
@@ -804,7 +678,7 @@ Proof.
     eapply (evalstar_ctx' es); S.inferContext; crush.
     simpl.
     eauto using termrel_proj₂, valrel_in_termrel.
-  - subst; eapply dwp_imprecise in dwp; subst.
+  - subst; eapply dwp_invert_imprecise in dwp; subst.
     eapply termrel_div_lt.
     eapply (divergence_closed_under_evalcontext' div); S.inferContext; crush.
   - eapply termrel_div_wrong.
@@ -871,7 +745,7 @@ Proof.
     eauto using emulate_pctx_T.  
   - induction scp; cbn;
     intros ts tu lr; 
-    rewrite ?S.pctx_cat_app;
+    rewrite ?S.pctx_cat_app, ?uvalApp_pctx₁_app, ?uvalApp_pctx₂_app;
     eauto using emulate_works, compat_emul_app, compat_emul_abs, compat_var, toEmulDV_entry, compat_emul_wrong', compat_emul_unit, compat_emul_true, compat_emul_false, compat_emul_pair, compat_emul_ite, compat_emul_inl, compat_emul_inr, compat_emul_proj₁, compat_emul_proj₂, compat_emul_seq, compat_emul_caseof;
     eapply compat_emul_caseof; crush;
     change (toEmulDV n p γ p▻ pEmulDV n p) with (toEmulDV n p (S γ));
