BackTrans/UValHelpers2.v
@@ -1,0 +1,193 @@
+Require Stlc.SpecSyntax.
+Require Utlc.SpecSyntax.
+Require Import BackTrans.UValHelpers.
+Require Import Stlc.SpecTyping.
+Require Import Stlc.StlcOmega.
+Require Import Stlc.LemmasTyping.
+Require Import Stlc.SpecEvaluation.
+Require Import Stlc.LemmasEvaluation.
+Require Import Utlc.SpecScoping.
+Require Import Utlc.LemmasScoping.
+Require Import Utlc.LemmasEvaluation.
+Require Import Utlc.DecideEval.
+Require Import LogRel.PseudoType.
+Require Import LogRel.LemmasPseudoType.
+Require Import LogRel.LR.
+Require Import LogRel.LemmasLR.
+Require Import LogRel.LemmasIntro.
+Require Import LogRel.LemmasInversion.
+Require Import Omega.
+Require Import Db.Lemmas.
+Require Import UVal.UVal.
+Require Utlc.Fix.
+Require Omega.
+
+Definition uvalApp_pctx₁ n ts₂ := S.papp₁ (S.papp₂ (S.abs (UVal n) (S.abs (UVal n) (S.app (caseArrUp n (S.var 1)) (S.var 0)))) S.phole) ts₂.
+Definition uvalApp_pctx₂ n ts₁ := S.papp₂ (S.app (S.abs (UVal n) (S.abs (UVal n) (S.app (caseArrUp n (S.var 1)) (S.var 0)))) ts₁) S.phole.
+Definition uvalApp n ts₁ ts₂ := S.app (S.app (S.abs (UVal n) (S.abs (UVal n) (S.app (caseArrUp n (S.var 1)) (S.var 0)))) ts₁) ts₂.
+
+(* Arguments uvalApp_pctx₁ n ts₂ : simpl never. *)
+(* Arguments uvalApp_pctx₂ n ts₁ : simpl never. *)
+(* Arguments uvalApp n ts₁ ts₂ : simpl never. *)
+
+Lemma uvalApp_T {n ts₁ ts₂ Γ} :
+  ⟪ Γ ⊢ ts₁ : UVal n ⟫ →
+  ⟪ Γ ⊢ ts₂ : UVal n ⟫ →
+  ⟪ Γ ⊢ uvalApp n ts₁ ts₂ : UVal n ⟫.
+Proof.
+  unfold uvalApp.
+  eauto with typing uval_typing.
+Qed.
+
+Lemma uvalApp_pctx₁_T {n ts₂ Γ} :
+  ⟪ Γ ⊢ ts₂ : UVal n ⟫ →
+  ⟪ ⊢ uvalApp_pctx₁ n ts₂ : Γ , UVal n → Γ , UVal n ⟫.
+Proof.
+  unfold uvalApp_pctx₁.
+  eauto with typing uval_typing.
+Qed.
+
+Lemma uvalApp_pctx₂_T {n ts₁ Γ} :
+  ⟪ Γ ⊢ ts₁ : UVal n ⟫ →
+  ⟪ ⊢ uvalApp_pctx₂ n ts₁ : Γ , UVal n → Γ , UVal n ⟫.
+Proof.
+  unfold uvalApp_pctx₂.
+  eauto with typing uval_typing.
+Qed.
+
+Hint Resolve uvalApp_T : uval_typing.
+Hint Resolve uvalApp_pctx₁_T : uval_typing.
+Hint Resolve uvalApp_pctx₂_T : uval_typing.
+
+Local Ltac crush :=
+  repeat (repeat crushUtlcSyntaxMatchH; 
+          repeat crushStlcSyntaxMatchH; 
+          repeat crushStlcEval; 
+          repeat crushUtlcEvaluationMatchH; 
+          repeat crushUtlcEvaluationMatchH2; 
+          repeat crushUtlcEvaluationMatchH2; 
+          repeat crushUtlcScopingMatchH;
+          repeat crushDbSyntaxMatchH;
+          repeat crushDbLemmasMatchH;
+          repeat crushDbLemmasRewriteH;
+          try assumption;
+          crushOfType;
+          trivial;
+          eauto using caseUnit_pctx_ECtx, caseBool_pctx_ECtx, caseProd_pctx_ECtx, caseSum_pctx_ECtx, caseArr_pctx_ECtx, upgrade_value, downgrade_value with typing
+         ).
+
+Lemma uvalApp_sub {n ts₁ ts₂ γ} :
+  (uvalApp n ts₁ ts₂) [γ] = uvalApp n (ts₁[γ]) (ts₂[γ]).
+Proof.
+  unfold uvalApp; cbn.
+  crush; rewrite caseArrUp_sub;
+  crush.
+Qed.
+
+Lemma termrel_uvalApp {d w n p ts₁ tu₁ ts₂ tu₂} :
+  dir_world_prec n w d p →
+  termrel d w (pEmulDV n p) ts₁ tu₁ →
+  (∀ w' : World, w' ≤ w → termrel d w' (pEmulDV n p) ts₂ tu₂) →
+  termrel d w (pEmulDV n p) (uvalApp n ts₁ ts₂) (U.app tu₁ tu₂).
+Proof.
+  intros dwp tr₁ tr₂.
+  unfold uvalApp, caseArrUp, caseArrUp_pctx.
+  (* evaluate ts₁ and tu₁ *)
+  eapply (termrel_ectx' tr₁); S.inferContext; U.inferContext; 
+  unfold pctx_cat, U.ECtx; crush.
+
+  (* continuation boilerplate *)
+  intros w' futw vs₁ vu₁ vr₁.
+  destruct (valrel_implies_OfType vr₁) as [[vvs₁ ?] [? ?]].
+  rewrite S.pctx_cat_app; cbn.
+
+  (* beta-reduce the outer let *)
+  eapply termrel_antired_eval_left.
+  eapply (S.eval_from_eval₀ (S.eval_beta vvs₁)); S.inferContext; crush.
+  cbn; crush.
+
+  (* bureaucracy *)
+  fold (caseArr n (S.app (upgrade n 1) (S.var 1))).
+  rewrite caseArr_sub; cbn; crush; rewrite upgrade_sub.
+
+  (* evaluate ts₂ and tu₂ *)
+  specialize (tr₂ w' futw).
+  eapply (termrel_ectx' tr₂); S.inferContext; U.inferContext; 
+  unfold pctx_cat, U.ECtx; crush.
+  
+  (* continuation boilerplate *)
+  intros w'' futw' vs₂ vu₂ vr₂.
+  destruct (valrel_implies_Value vr₂) as [vvs₂ ?].
+  cbn.
+
+  (* beta-reduce the remaining let *)
+  eapply termrel_antired_eval_left.
+  eapply (S.eval_from_eval₀ (S.eval_beta vvs₂)); S.inferContext; crush.
+  cbn; crush.
+
+  (* bureaucracy *)
+  fold (caseArr n (S.app (upgrade n 1) (S.var 1))).
+  rewrite ?caseArr_sub; cbn; crush; rewrite ?upgrade_sub.
+  rewrite <- ?ap_liftSub; rewrite -> ?liftSub_wkm; rewrite (apply_wkm_beta1_cancel vs₁ vs₂).
+  
+  (* execute the upgrade *)
+  assert (w'' ≤ w) by Omega.omega.
+  assert (valrel d w'' (pEmulDV n p) vs₁ vu₁) by eauto using valrel_mono.
+  assert (trupg : termrel d w'' (pEmulDV (n + 1) p) (S.app (upgrade n 1) vs₁) vu₁)
+    by (eauto using upgrade_works', dwp_mono).
+  unfold caseArr.
+  eapply (termrel_ectx' trupg); S.inferContext; U.inferContext; cbn; crush.
+
+  (* continuation bureaucracy *)
+  intros w''' futw'' vs₁' vu₁' vr₁'.
+  replace (n + 1) with (S n) in vr₁' by Omega.omega.
+
+  destruct (valrel_implies_Value vr₁').
+  (* case analysis *)
+  eapply invert_valrel_pEmulDV_for_caseUValArr in vr₁'.
+  destruct vr₁' as [(vs₁'' & ? & es & vr₁')|[(? & div)|(neq & div)]]; subst.
+  - (* Correct case *)
+
+    (* caseArr succeeds *)
+    eapply termrel_antired_star_left.
+    fold (caseArr n (inArr n vs₁'')).
+    eapply (evalstar_ctx' es); S.inferContext; crush.
+    cbn.
+
+    (* application works *)
+    eapply valrel_in_termrel in vr₁'.
+    eapply (termrel_app vr₁').
+
+    (* application argument is also fine *)
+    eauto using valrel_in_termrel, valrel_mono.
+  - (* unk case *) 
+    eapply dwp_invert_imprecise in dwp; subst.
+    eapply termrel_div_lt.
+    fold (caseArr n vs₁').
+    eapply (divergence_closed_under_evalcontext' div); S.inferContext; crush.
+  - (* other cases *)
+    
+    eapply termrel_div_wrong.
+    + fold (caseArr n vs₁').
+      eapply (divergence_closed_under_evalcontext' div); S.inferContext; crush.
+    + right.
+      eapply evalToStar.
+      eapply U.eval₀_to_eval.
+      eauto with eval.
+Qed.
+
+Lemma uvalApp_pctx₁_app {n ts₁ ts₂} :
+  S.pctx_app ts₁ (uvalApp_pctx₁ n ts₂) = uvalApp n ts₁ ts₂.
+Proof.
+  crush.
+Qed.
+
+Lemma uvalApp_pctx₂_app {n ts₁ ts₂} :
+  S.pctx_app ts₂ (uvalApp_pctx₂ n ts₁) = uvalApp n ts₁ ts₂.
+Proof.
+  crush.
+Qed.
+
+Arguments uvalApp_pctx₁ n ts₂ : simpl never.
+Arguments uvalApp_pctx₂ n ts₁ : simpl never.
+Arguments uvalApp n ts₁ ts₂ : simpl never.
