FullAbstraction.v
@@ -1,0 +1,112 @@
+Require Import Stlc.SpecTyping.
+Require Import Stlc.SpecEquivalent.
+Require Import Stlc.LemmasEvaluation.
+Require Import Stlc.LemmasTyping.
+Require Import Utlc.SpecEquivalent.
+Require Import Utlc.LemmasEvaluation.
+
+Require Import Compiler.Erase.
+Require Import Compiler.Compiler.
+Require Import Compiler.ProtectConfine.
+
+Require Import UVal.UVal.
+
+Require Import LogRel.PseudoType.
+Require Import LogRel.LemmasPseudoType.
+Require Import LogRel.LR.
+Require Import LogRel.LemmasLR.
+
+Require Import BackTrans.InjectExtract.
+Require Import BackTrans.UpgradeDowngrade.
+Require Import BackTrans.Emulate.
+
+Require Import Omega.
+
+Lemma equivalencePreservation {t₁ t₂ τ} :
+  ⟪ S.empty ⊢ t₁ : τ ⟫ →
+  ⟪ S.empty ⊢ t₂ : τ ⟫ →
+  ⟪ S.empty ⊢ t₁ ≃ t₂ : τ ⟫ →
+  ⟨ 0 ⊢ compile τ t₁ ≃ compile τ t₂ ⟩.
+Proof.
+  revert t₁ t₂ τ.
+  enough (∀ {t₁ t₂ τ}, 
+            ⟪ S.empty ⊢ t₁ : τ ⟫ →
+            ⟪ S.empty ⊢ t₂ : τ ⟫ →
+            ⟪ S.empty ⊢ t₁ ≃ t₂ : τ ⟫ →
+            ∀ {C}, ⟨ ⊢ C : 0 → 0 ⟩ →
+                 U.Terminating (U.pctx_app (compile τ t₁) C) → U.Terminating (U.pctx_app (compile τ t₂) C)) as Hltor
+      by (intros t₁ t₂ τ ty1 ty2 ceq;
+          assert (⟪ S.empty ⊢ t₂ ≃ t₁ : τ ⟫)
+            by (apply S.pctx_equiv_symm; assumption);
+          split;
+          refine (Hltor _ _ _ _ _ _ _ _); assumption).
+  intros t₁ t₂ τ ty₁ ty₂ ceq Cu sCu term.
+  
+  destruct (U.Terminating_TerminatingN term) as [n termN]; clear term.
+
+  assert (⟪ pempty ⊩ t₁ ⟦ dir_gt , S n ⟧ erase t₁ : embed τ ⟫) as lre₁
+      by (change pempty with (embedCtx (repEmulCtx pempty)); 
+          eapply erase_correct;
+          cbn; assumption).
+  assert (⟪ pempty ⊩ S.app (inject (S (S n)) τ) t₁ ⟦ dir_gt , S n ⟧ U.app (protect τ) (erase t₁) : pEmulDV (S (S n)) precise ⟫) as lrpe₁
+      by (eapply inject_works_open;
+          eauto using dwp_precise with arith).
+  fold (compile τ t₁) in lrpe₁.
+
+  assert (⟪ ⊩ emulate_pctx (S (S n)) Cu ⟦ dir_gt , S n ⟧ Cu : 
+              pempty , pEmulDV (S (S n)) precise → pempty , pEmulDV (S (S n)) precise ⟫) as lrem₁ by
+      (change pempty with (toEmulDV (S (S n)) precise 0);
+       eapply emulate_pctx_works; eauto using dwp_precise with arith).
+
+  pose proof (proj2 lrem₁ _ _ lrpe₁) as lrfull₁.
+
+  assert (S.Terminating (S.pctx_app (S.app (inject (S (S n)) τ) t₁)
+                                    (emulate_pctx (S (S n)) Cu))) as termS
+    by (eapply (adequacy_gt lrfull₁ termN); eauto with arith).
+
+  change (S.app (inject (S (S n)) τ) t₁) with (S.pctx_app t₁ (S.papp₂ (inject (S (S n)) τ) S.phole)) in termS.
+  rewrite <- S.pctx_cat_app in termS. 
+
+  assert (⟪ ⊢ emulate_pctx (S (S n)) Cu : S.empty, UVal (S (S n)) → S.empty, UVal (S (S n)) ⟫)
+    by (change S.empty with (toUVals (S (S n)) 0);
+        eapply emulate_pctx_T; assumption).
+
+  assert (S.Terminating (S.pctx_app t₂ (S.pctx_cat
+                 (S.papp₂ (inject (S (S n)) τ) S.phole)
+                 (emulate_pctx (S (S n)) Cu)))) as termS'
+    by (eapply ceq; eauto;
+        eapply pctxtyping_cat; crushTyping;
+        eauto using injectT, emulate_pctx_T).
+
+  destruct (S.Terminating_TerminatingN termS') as [m termSm']; clear termS'.
+
+  assert (⟪ pempty ⊩ t₂ ⟦ dir_lt , S m ⟧ erase t₂ : embed τ ⟫) as lre₂
+      by (change pempty with (embedCtx (repEmulCtx pempty)); 
+          eapply erase_correct;
+          cbn; assumption).
+  assert (⟪ pempty ⊩ S.app (inject (S (S n)) τ) t₂ ⟦ dir_lt , S m ⟧ U.app (protect τ) (erase t₂) : pEmulDV (S (S n)) imprecise ⟫) as lrpe₂
+      by (eapply inject_works_open;
+          eauto using dwp_imprecise).
+  fold (compile τ t₁) in lrpe₂.
+
+  assert (⟪ ⊩ emulate_pctx (S (S n)) Cu ⟦ dir_lt , S m ⟧ Cu : 
+              pempty , pEmulDV (S (S n)) imprecise → pempty , pEmulDV (S (S n)) imprecise ⟫) as lrem₂ by
+      (change pempty with (toEmulDV (S (S n)) imprecise 0);
+       eapply emulate_pctx_works; eauto using dwp_imprecise).
+
+  pose proof (proj2 lrem₂ _ _ lrpe₂) as lrfull₂.
+  rewrite S.pctx_cat_app in termSm'.
+
+  eapply (adequacy_lt lrfull₂ termSm'); eauto with arith.
+Qed.
+
+Lemma fullAbstraction {t₁ t₂ τ} :
+  ⟪ S.empty ⊢ t₁ : τ ⟫ →
+  ⟪ S.empty ⊢ t₂ : τ ⟫ →
+  ⟪ S.empty ⊢ t₁ ≃ t₂ : τ ⟫ ↔
+  ⟨ 0 ⊢ compile τ t₁ ≃ compile τ t₂ ⟩.
+Proof.
+  intros.
+  split;
+  eauto using equivalenceReflection, equivalencePreservation.
+Qed.
